cfi/symbolic.v
@@ -489,7 +489,169 @@ Program Instance symbolic_cfi_machine : cfi_machine := {|
   stopping := stopping  
  |}.
 
+Import DoNotation.
+Import Vector.VectorNotations.
 
+(*TODO: Move to symbolic*)
+Definition build_mvec st : option (Symbolic.MVec (Symbolic.tag t)) :=
+  let '(Symbolic.State mem reg pc@tpc int) := st in
+  match get mem pc with
+    | Some i =>
+      match decode_instr (common.val i) with
+        | Some op =>
+          let part := @Symbolic.mkMVec (Symbolic.tag t) (opcode_of op) tpc (tag i) in
+          match op return (Symbolic.mvec_operands (Symbolic.tag t) (Symbolic.nfields (opcode_of op)) ->
+                           Symbolic.MVec (Symbolic.tag t)) -> option (Symbolic.MVec (Symbolic.tag t)) with
+            | Nop => fun part => Some (part [])
+            | Const n r => fun part => 
+                do! old <- get reg r;
+                Some (part [tag old])
+            | Mov r1 r2 => fun part =>
+              do! v1 <- get reg r1;
+              do! v2 <- get reg r2;
+              Some (part [(tag v1); (tag v2)])
+            | Binop _ r1 r2 r3 => fun part =>
+              do! v1 <- get reg r1;
+              do! v2 <- get reg r2;
+              do! v3 <- get reg r3;
+              Some (part [(tag v1); (tag v2); (tag v3)])
+            | Load  r1 r2 => fun part =>
+              do! w1 <- get reg r1;
+              do! w2 <- get mem (val w1);
+              do! old <- get reg r2;
+              Some (part [(tag w1); (tag w2); (tag old)])
+            | Store  r1 r2 => fun part =>
+              do! w1 <- get reg r1;
+              do! w2 <- get reg r2;
+              do! w3 <- get mem (val w1);
+              Some (part [(tag w1); (tag w1); (tag w3)])
+            | Jump  r => fun part =>
+              do! w <- get reg r;
+              Some (part [tag w])
+            | Bnz  r n => fun part =>
+              do! w <- get reg r;
+              Some (part [tag w])
+            | Jal  r => fun part =>
+              do! w <- get reg r;
+              do! old <- get reg ra;
+              Some (part [tag w; tag old])
+            | JumpEpc => fun _ => None
+            | AddRule => fun _ => None
+            | GetTag _ _ => fun _ => None
+            | PutTag _ _ _ => fun _ => None
+            | Halt => fun _ => None
+          end part
+        | None => None
+      end
+    | None => 
+      match Symbolic.get_syscall table pc with
+        | Some sc =>
+          Some (@Symbolic.mkMVec (Symbolic.tag _) SERVICE tpc (Symbolic.entry_tag sc) (Vector.nil _))
+        | None => None
+      end 
+  end.
+
+Definition option_handler x := 
+  match x with
+    | Some v => Symbolic.handler v
+    | None => None
+  end.
+
+Lemma succ_false_handler asi asj :
+  invariants asi ->
+  ssucc asi asj = false ->
+  step asi asj ->
+  option_handler (build_mvec asj) = None.
+Proof.
+  intros INV SUCC STEP.
+  unfold ssucc in SUCC.
+  inv STEP; simpl in *;
+  rewrite PC in SUCC; try rewrite INST in SUCC;
+  repeat (
+      match goal with
+        | [H: Symbolic.next_state_pc _ _ _ = _ |- _] => 
+          unfold Symbolic.next_state_pc in H
+        | [H: Symbolic.next_state_reg _ _ _ _ = _ |- _] => 
+          unfold Symbolic.next_state_reg in H
+        | [H: Symbolic.next_state_reg_and_pc _ _ _ _ _ = _ |- _] => 
+          unfold Symbolic.next_state_reg_and_pc in H
+        | [H: Symbolic.next_state _ _ _ = Some _ |- _] =>
+          unfold Symbolic.next_state in H; simpl in H
+      end); match_inv; subst; simpl in SUCC;
+  try match goal with 
+        | [H: _ || _ = false |- _] => 
+          apply orb_false_iff in H;
+            destruct H as [? ?];
+            destruct (w == 0);
+            unfold pc' in *
+      end;
+  try match goal with
+        | [H: (?A == ?A) = false |- _] => 
+      move/eqP:H => CONTRA; destruct (CONTRA erefl)
+      end;
+  simpl;
+  repeat match goal with
+    | [ |- option_handler match get ?Mem ?W with _ => _ end = _] => 
+      destruct (get Mem W) eqn:GET
+    | [ |- option_handler match decode_instr (val ?I) with _ => _ end = _] => 
+      destruct (decode_instr (val I)) 
+  end; try (destruct i0);
+  try match goal with
+    | [|- option_handler None = None] => unfold option_handler; reflexivity
+  end; 
+  destruct INV as [ITG [VTG ETG]]; simpl in *;
+  unfold option_handler; simpl;
+  try match goal with
+    | |- context[get ?Reg ?R] => destruct (get Reg R)
+         end;
+  try match goal with
+        | |- context[Some ?A] => destruct A; simpl
+      end;
+  try match goal with
+    | |- context[get ?Reg ?R] => destruct (get Reg R)
+         end;
+  try match goal with
+        | |- context[Some ?A] => destruct A; simpl
+      end;
+  try match goal with
+        | |- context[get ?Reg ?R] => destruct (get Reg R)
+      end;
+  try match goal with
+        | |- context[Some ?A] => destruct A; simpl
+      end;
+  try match goal with
+    | [H: valid_jmp ?Pc ?W = false, H1: get ?Mem ?W = Some ?A |- _ ] =>
+       destruct a as [v tg]; simpl;
+       destruct tg as [[id|] |]; try reflexivity
+  end;
+ try match goal with
+    | [|- match match ?Expr with _ => _ end with _ => _ end = None] => destruct Expr eqn:GETCALL
+  end;
+  unfold entry_points_tagged in ETG;
+  try match goal with
+        |[H: Symbolic.get_syscall _ _ = Some ?Sc |- _] =>
+         destruct (Symbolic.entry_tag Sc) as [[id|]|] eqn:ETAG
+      end;
+  try reflexivity;
+  try match goal with
+    | [H: get ?Mem ?Pc = Some ?I@(INSTR (Some ?S)), H1: valid_jmp ?Pc ?W = false,
+       H2: get ?Mem ?W = None,                                                 
+       H3: Symbolic.get_syscall _ ?W  = Some ?Sc,
+       H4: Symbolic.entry_tag _ = INSTR (Some _) |- _ ] =>
+       assert (TG := ITG _ _ _ H); subst;
+       assert (TG := ETG _ _ _ H2 H3 H4); subst;
+       simpl; rewrite H1
+    end;
+  try match goal with
+    | [H: get ?Mem ?Pc = Some ?I@(INSTR (Some ?S)), H1: valid_jmp ?Pc ?W = false,
+       H2: get ?Mem ?W  = Some _@(INSTR (Some ?Id)) |- _ ] =>
+       assert (TG := ITG _ _ _ H); subst;
+       assert (TG := ITG _ _ _ H2); subst;
+       rewrite H1
+       end;
+  try reflexivity;
+  try (destruct tag1; reflexivity).
+Qed.
 
 End WithClasses.
 
